More definitions and operators for delta correctness.

Security/SaberRqDeltaCorrectness.ec
@@ -115,13 +115,189 @@ op cmq_expression (_A : Rq_mat) (s s': Rq_vec) (m : R2) : Rq =
   let v' = v'_expression _A s s' in
   v' + (scaleR22Rq m) + error_cmq _A s s' m.
 
-op m'_expression (_A : Rq_mat) (s s': Rq_vec) (m : R2) : R2 =
+op m'_expression_Rq (_A : Rq_mat) (s s': Rq_vec) (m : R2) : Rq =
   let v = v_expression _A s s' in
   let cmq = cmq_expression _A s s' m in
-  scaleRq2R2 (v - cmq + (upscaleRq h2 (eq - ep))).
+  v - cmq + (upscaleRq h2 (eq - ep)).
 
+op m'_expression (_A : Rq_mat) (s s': Rq_vec) (m : R2) : R2 = scaleRq2R2 (m'_expression_Rq _A s s' m).
 
+pragma Goals:printall.
 
+lemma errrng_impl_correct_Zq (m : Z2) (err : Zq) :
+  0 <= Zq.asint err < q %/ 2 => m = scaleZq2Z2 (scaleZ22Zq m + err).
+proof.
++ case => [ge0_err @/q]; rewrite (_ : 2 ^ eq = 2 ^ (eq - 1) * 2) 2:mulzK // => [| ltq2_err].
+  - by rewrite -{3}expr1 -exprD_nneg; smt(ge3_eq). 
+  rewrite /scaleZq2Z2 /scaleZ22Zq /downscale /upscale /shr /shl !inzmodK modzDml /q modz_pow2_div;
+          1, 2 : smt(Z2.ge0_asint Zq.ge0_asint addr_ge0 mulr_ge0 expr_ge0 ge3_eq).
+  rewrite opprD addzA /= expr1 /inzmod modz_mod divzMDl; 1: rewrite neq_ltz expr_gt0 //=.
+  have -> /=: asint err %/ 2 ^ (eq - 1) = 0 by rewrite pdiv_small.
+  by rewrite -{1}asintK /inzmod.
+qed.
+
+lemma correct_impl_errrng_Zq (m : Z2) (err : Zq) :
+   m = scaleZq2Z2 (scaleZ22Zq m + err) => 0 <= Zq.asint err < q %/ 2.
+proof.
+have h /h errd0: m = scaleZq2Z2 (scaleZ22Zq m + err) => Zq.asint err %/ 2 ^ (eq - 1) = 0; last first.
++ rewrite /q (_ : 2 ^ eq = 2 ^ (eq - 1) * 2) 2:mulzK //. 
+  - rewrite -{3}expr1 -exprD_nneg; smt(ge3_eq).
+  by rewrite -divz_eq0 in errd0; 1: rewrite expr_gt0 //.
++ rewrite /scaleZq2Z2 /scaleZ22Zq /downscale /upscale /shr /shl !inzmodK modzDml /q modz_pow2_div;
+          1, 2 : smt(Z2.ge0_asint Zq.ge0_asint addr_ge0 mulr_ge0 expr_ge0 ge3_eq).
+  rewrite opprD addzA /= expr1 /inzmod modz_mod divzMDl; 1: rewrite neq_ltz expr_gt0 //.
+  rewrite -{1}asintK -eq_inzmod.
+  case (asint err < 2 ^ (eq - 1)); [move: (Zq.ge0_asint err) | move: (Zq.gtp_asint err)]
+       => [ge0_err ltq2_err _ | @/q ltq_err /lezNgt geq2_err].
+  - by rewrite -divz_eq0 1:expr_gt0.  
+  - have -> /=: asint err %/ 2 ^ (eq - 1) = 1.
+    * rewrite eqz_leq -(ler_add2l 1) lez_add1r /= ltz_divLR 2:lez_divRL 1,2:expr_gt0 //=.
+      rewrite -{1}expr1 -exprD_nneg //; smt(ge3_eq).
+    move: (Z2.rg_asint m); rewrite andabP andbC -lez_add1r -(lez_add2r (-1)) /=; case => le1m ge0m.
+    case (asint m = 0) => [-> //| /neq_ltz [/ltzNge // |]].
+    * rewrite -lez_add1r /= => ge1m; have -> //: asint m = 1 by rewrite eqz_leq.
+qed.
+
+lemma correct_errrng_Zq (m : Z2) (err : Zq) :
+ 0 <= Zq.asint err < q %/ 2 <=> m = scaleZq2Z2 (scaleZ22Zq m + err).
+proof. by split; [apply errrng_impl_correct_Zq | apply correct_impl_errrng_Zq]. qed.
+
+lemma correct_errrng_Rq (m : R2) (err : Rq) :
+ (forall (i : int), 0 <= i < n => 0 <= Zq.asint err.[i] < q %/ 2)
+ <=> 
+ (m = scaleRq2R2 (scaleR22Rq m + err)).
+proof.
+split; rewrite polyXnD1_eqP => [coeff_errrng i rng_i | corr i rng_i]; 2: move: (corr i rng_i);
+       rewrite rcoeffZ_sum //= rcoeffD rcoeffZ_sum //=.
++ by move: (coeff_errrng i rng_i); apply errrng_impl_correct_Zq.
++ by apply correct_impl_errrng_Zq.
+qed.
+
+lemma test0 (_A : Rq_mat) (s s' err: Rq_vec) :
+ (dotp (trmx _A *^ s' + err) s) = (dotp (_A *^ s) s' + dotp err s).
+proof. by rewrite dotpDl dotpC mulmxTv -dotp_mulmxv. qed.
+
+lemma test1 (_A : Rq_mat) (s s': Rq_vec) (err err': Rq_vec) :
+  (dotp (trmx _A *^ s' + err') s) - (dotp (_A *^ s + err) s')
+  =
+  dotp err' s - dotp err s'.
+proof.
+rewrite test0 addrC. rewrite dotpDl.
+pose dass' := dotp (_A *^ s) s'; pose derrs' := dotp err s'; pose derrs := dotp err' s.
+rewrite addrC. 
+rewrite eq_sym addrC. 
+rewrite opprD. rewrite addrA. rewrite eq_sym. rewrite addrC.
+rewrite &(Rq.ComRing.addrI derrs'). rewrite addrA eq_sym addrA. simplify.
+rewrite subrr.
+rewrite 2!add0r.
+rewrite eq_sym -addrA addrC -addrA.
+rewrite &(Rq.ComRing.addrI (-derrs)).
+rewrite addrA.
+rewrite addrC eq_sym addrC subrr addr0.
+rewrite addrC eq_sym subr_eq0 //.
+qed.
+
+op m'_expression_reduced (_A : Rq_mat) (s s': Rq_vec) (m : R2) : R2 =
+  scaleRq2R2 (
+  dotp (error_bq' _A s') s - dotp (error_bq _A s) s' 
+  - scaleR22Rq m - error_cmq _A s s' m + upscaleRq h2 (eq - ep)).
+
+instance ring with Rq
+  op rzero = Rq.zeroXnD1
+  op rone  = Rq.oneXnD1
+  op add   = Rq.( + )
+  op opp   = Rq.([-])
+  op mul   = Rq.( * )
+  op expr  = Rq.ComRing.exp
+  op ofint = Rq.ComRing.ofint
+
+  proof oner_neq0 by apply Rq.ComRing.oner_neq0
+  proof addrA     by apply Rq.ComRing.addrA
+  proof addrC     by apply Rq.ComRing.addrC
+  proof addr0     by apply Rq.ComRing.addr0
+  proof addrN     by apply Rq.ComRing.addrN
+  proof mulr1     by apply Rq.ComRing.mulr1
+  proof mulrA     by apply Rq.ComRing.mulrA
+  proof mulrC     by apply Rq.ComRing.mulrC
+  proof mulrDl    by apply Rq.ComRing.mulrDl
+  proof expr0     by apply Rq.ComRing.expr0
+  proof ofint0    by apply Rq.ComRing.ofint0
+  proof ofint1    by apply Rq.ComRing.ofint1
+  proof exprS     by apply Rq.ComRing.exprS
+  proof ofintS    by apply Rq.ComRing.ofintS
+  proof ofintN    by apply Rq.ComRing.ofintN.
+
+lemma test (_A : Rq_mat) (s s': Rq_vec) (m : R2) :
+  m'_expression _A s s' m = m'_expression_reduced _A s s' m.
+proof.
+rewrite /m'_expression /m'_expression_Rq /v_expression /cmq_expression 
+        /v'_expression /m'_expression_reduced /=.
+congr. 
+congr.
+ring.
+rewrite addrC.
+rewrite test0.
+ring.
+rewrite dotpDl. ring.
+qed.
+
+lemma scaleZ22Zq_PN (z : Z2) : scaleZ22Zq z = scaleZ22Zq (- z).
+proof.
+rewrite /scaleZ22Zq /upscale /shl -eq_inzmod !inzmodK; do 3! congr.
+case (asint z = 0) => [-> //| /neq_ltz [lt0_z | gt0_z]]; move: (Z2.rg_asint z); case => ge0_z lt2_z.
++ by rewrite ltzNge in lt0_z.
++ rewrite -lez_add1r -(lez_add2l (-1)) /= in lt2_z; rewrite -lez_add1r /= in gt0_z.
+  by move: (eqz_leq (asint z) 1); rewrite gt0_z lt2_z /= => ->.
+qed.
+
+lemma scaleR22Rq_PN (p : R2) : scaleR22Rq p = scaleR22Rq (- p).
+proof.
+rewrite /scaleR22Rq !BigRq.XnD1CA.big_seq &(BigRq.XnD1CA.eq_bigr) /= => *.
+by rewrite -rcoeffN scaleZ22Zq_PN.
+qed.
+
+lemma scaleZ22Zq_N (z : Z2) : scaleZ22Zq (- z) = - scaleZ22Zq z.
+proof.
+rewrite /scaleZ22Zq /upscale /shl -inzmodN oppE -eq_inzmod /q -modz_pow2_mul; 1: smt(ge3_eq).
+rewrite expr1 modz_mod -{1}(Ring.IntID.expr1 2) modz_pow2_mul; 1: smt(ge3_eq).
+by rewrite mulNr.
+qed.
+
+lemma scaleR22Rq_N (p : R2) : scaleR22Rq (- p) = - scaleR22Rq p.
+proof.
+rewrite /scaleR22Rq Rq.polyXnD1_sumN /= !BigRq.XnD1CA.big_seq &(BigRq.XnD1CA.eq_bigr) /= => *.
+by rewrite -rcoeffN scaleZ22Zq_N scaleN.
+qed.
+
+(*
+lemma test12 (_A : Rq_mat) (s s': Rq_vec) (m : R2):
+  m = m'_expression _A s s' m.
+proof.
+rewrite test.
+rewrite /m'_expression_reduced.
+rewrite scaleRq2R2_DM.
+rewrite /v_expression.
+simplify.
+rewrite /cmq_expression.
+rewrite /v'_expression.
+simplify.
+have ->:
+(dotp (_A *^ s) s' + dotp (error_bq' _A s') s + upscaleRq h1 (eq - ep) -
+    (dotp (_A *^ s + error_bq _A s) s' + upscaleRq h1 (eq - ep) +
+     scaleR22Rq m + error_cmq _A s s' m))
+=
+(dotp (_A *^ s) s' + dotp (error_bq' _A s') s + upscaleRq h1 (eq - ep) -
+    dotp (_A *^ s + error_bq _A s) s' - upscaleRq h1 (eq - ep) -
+     scaleR22Rq m + error_cmq _A s s' m).
+
+have ->: (dotp (trmx _A *^ s' + error_bq' _A s') s = (dotp (_A *^ s) s' + dotp (error_bq' _A s') s)).
+rewrite test0 //.
+rewrite {1}test1.
+qed.
+ 
+lemma rel_m_m' (m : R2) (er : int):
+ - (q %/ 4) <= er < q %/ 4 => m = scaleRq2R2 (scaleR22Rq m + Rq.inzmod er).
+*)
 (* 
 bq <- scaleRpv2Rqv b;
 b <- scaleRqv2Rpv (_A *^ s + h)
@@ -145,6 +321,4 @@ v <- (dotp bq' s) + (upscaleRq h1 (eq - ep))
 
 
 *)
-op error_expression () : 
-
 
